#### Hedging for $$T = 1$$

Consider the following example, where we try to hedge $$X$$ at $$T = 1$$. That is, we are trying to find a strategy $$\phi = (\alpha_!, \beta_1)$$ such that $$V_1(\phi) = \alpha_1 S_1 + \beta_1 B_1\equiv X$$. 

We have two cases based on the stock movement -

- $$\alpha_1 S_0 u + \beta_1 (1 + r) = X^u$$
- $$\alpha_1 S_0 d + \beta_1 (1 + r) = X^d$$

Equivalently, $$\alpha_1 S_o(u - d) = X^u - X^d$$

$$
\begin{align*}
\alpha_1 &= \frac{X^u - X^d}{u - d}\frac{1}{S_0} \\
 \beta_1 &= \frac{uX^u - d X^d}{u - d}\frac{1}{B_1}
 \end{align*}
$$




Consequently, 

$$
\begin{align*}
V_0 (\phi) = \alpha_1 S_0 + \beta_1 \\
&= \frac{X^u - X^d}{u- d} + \frac{uX^d - d X^u}{u - d}\frac{1}{1 + r} \\
&= \frac{1}{1 + r}\left\{X^u \left(\frac{1 + r - d}{u - d}\right) + X^d \left(\frac{u - 1 - r}{u - d}\right)\right\} \\
&= \frac{1}{1 + r} \mathbb E^* (X)
\end{align*}
$$

The above expression is reminiscent of an expectation formulation where $$p^* = \frac{1 + r - d}{u - d}$$ and $$0 < p^* < 1$$. Here, the set $$\{S_), S_1/(1 + r)\}$$ is $$p^*$$-martingale.

What is a Martingale? A Martingale is a sequence of random variables representing a stochastic process for which, at a particular time, the conditional expectation of the next value in the sequence is equal to the present value, regardless of all prior values.

In the above case, we have 

$$
\begin{align*}
\mathbb E^* (S_1/(1 + r) \vert \mathcal F_0) &= S_0 u p^* + S_0 d(1 - p)^* \\
&= S_0 \implies \mathbb E^*(S_1) = S_0(1 + r)
\end{align*}
$$



**Theorem 1 (T = 1)** *For a given $$X$$, the value $$\mathbb E^*(X)/(1 + r)$$ is the non-arbitrage price of $$X$$ at $$t = 0$$.* 
That is, if $$C_0$$ is the market price of $$X$$, then $$V_0 = \mathbb E^*(X)/(1 + r) = V_0(\bar phi)$$ where $$\bar \phi = (\bar \alpha_1, \bar \beta_1)$$ (the values we calculated before). Consider the following cases - 

1. Say $$C_0 > V_0$$
    To make an arbitrage in this situation, we sell $$X$$ for $$C_0$$. We invest $$V_0$$ in the stock and $$C_0 - V_0 > 0$$ in the bond at $$t = 0$$. At time $$t = 1$$, we get $$V_1(\bar \phi) = X$$ yielding $$(C_0 - V_0)(1 + r) > 0 $$ as profit from the bond.

2. Say $$C_0 < V_0$$
    We do the opposite from above, where we buy the asset $$X$$. Short sell $$\bar \phi$$ for $$V_0$$, and invest $$C_0$$ in $$X$$ and $$V_0 - C_0$$ in the bond. We get the profit $$(V_0 - C_0)(1 + r)$$ at $$t = 1$$.

3. Say $$C_0 = V_0$$
    Here, we can show that no one can make an arbitrage. Consider the strategy $$\psi = (\alpha_1, \beta_1, \gamma_1)$$ where $$\gamma_1$$ is the contingent claim. We need to argue that no arbitrage can be made with any such strategy. We have,
   
   $$
   \begin{align*}

 V_0(\psi) &= \alpha_1 S_0 + \beta_1 + \gamma_1 C_0 \\
 V_1(\psi) &= \alpha_1 S_1 + \beta B_1 + \gamma_1 X \\
 \implies \mathbb E^*(V_1(\psi)) &= \mathbb E^*(\alpha_1 S_1 + \beta_1 B1 + \gamma_1 X) \\
 &= \alpha_1 \mathbb E^*(S_1) + \beta_1 (1 + r) + \gamma_1 \mathbb E^*(X)
\end{align*}
   $$
   
   
   
   
    We can distribute the expectation this way due to the linearity property. Recall that, we typically assume $$B_0 = 1$$ for brevity. Continuting the calculations,
   
   $$
   \begin{align*}

 \mathbb E^*(V_1(\psi)) &= \alpha_1 S_1(1 + r) + \beta_1(1 + r) + \gamma_1 V_0 (\bar \phi)(1 + r) \\
 &= \alpha_1 S_1(1 + r) + \beta_1(1 + r) + \gamma_1 C_0 (1 + r) \\
 &= (1 + r) V_0 (\psi)

\end{align*}
   $$
   
   
   
    IF $$V_0(\psi) = 0$$, then $$\mathbb E^*(V_1(\psi)) = 0$$, and if $$V_1(\psi) \geq 0 $$, then $$P^*(V_1(\psi) = 0) = 1$$. That is, $$V_1(\psi) = 0$$ meaning no arbitrage can be made with any strategy $$\psi$$. 

#### General $$T$$

This analysis can be extended to derive the hedging strategy a general $$t > 1$$. Given an $$X$$, find $$\phi = \{(\alpha_t, \beta_t): t = 1, \dots, T\}$$ such that $$V_T(\phi) = X$$ (resulting in $$C_0 = V_0(\phi)$$). To derive such a strategy, we work backwards in time starting from $$V_T(\phi) = X$$. This way, we can also calculate the intermediate price - the price to enter the market at some intermediary time $$t$$. It is helpful to think of the tree visualization for the price evolution.

$$
\begin{align*}
    V_T(\phi) = \alpha_T S_T + \beta_T B_T = X
\end{align*}
$$

conditional on $$\mathcal F_{T - 1}$$. Focusing on $$T - 1$$ and $$T$$, the analysis is similar to the previous case wherein $$X^U = X(w_1 \dots w_{T - 1} u)$$ and $$X^d = X(w_1 \dots w_{T - 1} d)$$. Doing so we get

$$
\left.
\begin{align*}
\alpha_T = \frac{X^u - X^d}{u - d}\frac{1}{S_{T - 1}} \\
\beta_T = \frac{uX^d - dX^u}{u - d}\frac{1}{(1 + r)^T}
\end{align*} \right\} \in \mathcal F_{T - 1} 
$$

Using the property of Martingales, 

$$
\begin{align*}
\mathbb E^* (X \vert \mathcal F_{T - 1}) = \mathbb E^* [V_T(\phi) \vert \mathcal F_{T - 1}]
&= \mathbb E^*[\alpha_T S_T + \beta_T B_T \vert \mathcal F_{T - 1}] \\
&= \alpha_T \mathbb E^*(S_T \vert \mathcal F_{T - 1}) + \beta_T B_T  \\
&= \alpha_T \left(p^* S_{T - 1} u + (1 - p^*) S_{T - 1} d\right) + \beta_T B_T \\
&= \alpha_T S_{T - 1}(1 + r) + \beta_T B_T
\end{align*}
$$

*Note.* $$\alpha_T, \beta_T$$ are constants with respect to the *condition* $$\mathcal F_{T - 1}$$, and that is why the linearity property can be used.  
