To summarise, for a payout random variable $$Y = \{Y_0, \dots, Y_T\}$$, we have $$U_t$$ as the necessary wealth at each time $$t$$. Then, the super-hedging strategy $$\phi^*$$ has the following properties -

- $$V^*_t(\phi^*)$$ is a martingale

- $$V^*(\phi^*) \geq U^*_t \geq Y^*_t$$ for all $$t$$

We define $$\bar \tau$$ such that $$\bar \tau = \min\{t \vert U_t = Y_t) \wedge T$$. With this definition, we have

$$
V_t^*(\phi^*) = U_t^*
$$

for $$t = 0, 1, \dots, \bar \tau$$ and $$V_0(\phi^*) = U_0$$. 

**Theorem.** $$U_0$$ is the no-arbitrage price for American call option based on $$Y$$. 

*Proof.*

1. $$C_0 > U_0$$, then there's arbitrage for the seller. The seller sells the claim for $$C_0$$ and buys $$\phi^*$$ for $$U_0$$. The remaining amount, $$C_0 - U_0$$ is invested in bonds. Then, for this strategy $$\phi^s$$, we have
   
   $$
   \begin{align*}
V_t(\phi^s) &= V_t(\phi^*)+ (C_0 - U_))B_t \\
V_\tau(\phi^s &= V_\tau(\phi^*) + \underbrace{(C_0 - U_0)B_\tau}_{>0} \\
&\geq U_\tau + \dots \\
&\geq Y_\tau + \dots
\end{align*}
   $$

2. $$C_0 < U_0$$, we have a buyer's arbitrage for the strategy $$\phi^b$$
   
   $$
   \phi^b = \begin{cases} -U_0 & \text{in } -\phi^* \\ U_0 - C_0 & \text{in bond} \end{cases}
   $$
   
   Then,
   
   $$
   \begin{align*}
V_0(\phi^b) &= -C_0 \\
V_\tau(\phi^b) &= - V_\tau(\phi^*) + (U_0 - C_0)B_\tau 
\end{align*}
   $$
   
   Using $$\tau = \bar \tau$$,
   
   $$
   \begin{align*}
V_{\bar \tau}(\phi^b) + Y_{\bar \tau} &= -V_{\bar \tau}(\phi^*) + (U_0 - C_0)B_{\bar \tau} + Y_{\bar \tau} \\
&= (U_0 - C_0) B_{\bar \tau} > 0
\end{align*}
   $$

3. $$C_0 = U_0$$. We need to show separately that there's no seller's and buyer's arbitrage
   
   1. No seller's arbitrage - Suppose $$\phi^s$$ is a seller's arbitrage strategy. We have
      
      $$
      V_0(\phi^s) = C_0, V_\tau(\phi^s) \geq Y_\tau
      $$
      
      Note that all elements need not be strictly greater for an arbitrage. Computing the expectation,
      
      $$
      \mathbb E^*(Y^*_\tau) < \mathbb E^*(V^*_\tau(\phi^s)) = V_0(\phi^s) = U_0 = C_0
      $$
      
      for all stopping times $$\tau$$. However, 
      
      > why strictly less than in the above equation?
      
      $$
      \mathbb E^*(Y^*_\tau) = \mathbb E^*(V_\tau^*(\phi^s)) = V_0(\phi^s) = C_0
      $$
      
      This shows that no seller's arbitrage is possible.
   
   2. No buyer's arbitrage - Suppose $$\phi^b$$ is such that 
      
      $$
      \begin{align*}
V_0(\phi^b) &= -C_0 \\
\exists \tau_0 V_{\tau_0} (\phi^b) + Y_{\tau_0} &\geq 0 \quad (> 0 \text{ sometimes})
\end{align*}
      $$
      
      Then, computing the expectation
      
      $$
      \begin{align*}
\mathbb E^*(V^*_\tau(\phi^b)) &= V_0(\phi^b) = -C_0 \\
\mathbb E^*(V_\tau^*(\phi^b) + Y_\tau^*) &= -C_0 + \mathbb E^*(Y^*_\tau) \\
&\leq -C_0 + \mathbb E^*(U^*_\tau) \\
& \leq -C_0 + U_0 = 0
\end{align*}
      $$
      
      This shows that no buyer's arbitrage is possible. $$\square$$

### Example

Consider anMerican Call $$S_0 = 4, r = 0.25, u = 2, d = 0.5, K = 4, T = 3$$. This yields $$p^* = 0.5$$. We have the following 

$$
S_t \implies \begin{align*}
&4 \\
2 &\quad 8 \\
1 \quad &4 \quad 16 \\
0.5 \quad 2 &\quad 8 \quad 32

\end{align*}
$$

$$
Y_t \implies \begin{align*}
&0 \\
0 &\quad 4 \\
0 \quad &0 \quad 12 \\
0 \quad 0 &\quad 0 \quad 28

\end{align*}
$$

$$
U_t = V_t \implies \begin{align*}
&\frac{64}{5} \\
\frac{16}{25} &\quad \frac{144}{25} \\
0 \quad &\frac{8}{5} \quad \frac{64}{5} \\
0 \quad 0 &\quad 4 \quad 28

\end{align*}
$$

## American Call-Put Parity

The relation between call and put options in general can be shown using **Jensen's inequality**. We have 

$$
\begin{align*}
\mathbb E(\phi(X)) &\geq \phi(\mathbb E(X)) \\
\mathbb E(\phi(X \vert \mathcal G)) &\geq \phi(\mathbb E(X | \mathcal G)) 
\end{align*}
$$

The payout functions for both call and put options are convex. We aim to show that $$U_t = V_t$$ for $$t = T, T - 1, \dots, 1, 0$$, using induction. The statement is true for $$t = T$$.

ASsume $$U_s = V_s $$ for $$s = t, t + 1, \dots, T$$, then

$$
\begin{align*}
U_{t - 1} &= \max \left(Y_{t - 1} , \frac{1}{1 + r} \mathbb E^*(U_t \vert \mathcal F_{T - 1})\right)\\
&=  \max \left(Y_{t - 1} , \frac{1}{1 + r} \mathbb E^*(V_t \vert \mathcal F_{T - 1})\right)\\
\end{align*}
$$

Substituting $$V_t = \frac{1}{(1 + r)^{T - \tau}} \mathbb E^*(V_t \vert \mathcal F_t)$$, 

$$
\begin{align*}
\mathbb E^*(V_t \vert \mathcal F_{t - 1}) &= \frac{1}{(1 + r)^{T - t}} \mathbb E^*(V_T \vert \mathcal F_{t - 1}) \\
&= \frac{1}{(1 + r)^{T - t}} \mathbb E^*((S_T - K)^+ \vert \mathcal F_{T - 1}) \\
&\geq \frac{1}{(1 + r)^{T - t}} \left(\mathbb E^*(S_T \vert \mathcal F_{t - 1}) - K\right)^+  & \because \text{Jensen's inequality}\\
&= \frac{1}{(1 + r)^{T - t}} ((1 + r)^{T - t + 1}S_{t - 1} - K)^+ \\
&= (1 + r)\left( S_{t - 1} - \frac{K}{(1 + r)^{T - t + 1}}\right)^+ \\
&\geq (1 + r) (S_{t - 1} - K)^+ \\
&= (1 + r) Y_{t - 1}
\end{align*}
$$



Using this result above, we have

$$
\begin{align*}
U_{t - 1} &= \max \left(Y_{t - 1} , \frac{1}{1 + r} \mathbb E^*(V_t \vert \mathcal F_{T - 1})\right)\\
&=  \frac{1}{1 + r} \mathbb E^*(V_t  \vert \mathcal F_{T - 1}) = V_{t - 1}
\end{align*}
$$


