For $\alpha > 0$, we let $\frac{1}{\beta} = \mathbb E(\alpha^{\xi_k}) = \alpha p + \frac{1}{\alpha}(1 - p)$. Then,

$$
\begin{align*}
\mathbb E(M_{n + 1} \vert \mathcal F_n) &= \alpha^{X_n} \beta^{n + 1} \mathbb E(\alpha^{\xi_{n + 1}} \vert \mathcal F_n) \\
&= \alpha^{X_n} \beta^{n + 1} \frac{1}{\beta} = \alpha^{X_n} \beta_n = M_n
\end{align*}
$$

That concludes the proof.

**Claim.** When $p \geq \frac{1}{2}$, then $P_x(\tau_b < \infty) = 1$ where $\tau_a = \min(n \geq 0: X_n = a)$ ($=\infty$ if no such $n$).  Note that we are not dealing with finite timeframe anymore.

The graph of $\beta$ looks like

*Proof.* So for $b \geq X$, we choose $0 < \alpha < 1$ such that $\beta > 1$, then

$$
\begin{align*}
\alpha^X &= \mathbb E_X(M_{n \wedge \tau_b}) \\
&= \mathbb E_X(\alpha^{X_{n \wedge \tau_b}} \beta^{n \wedge \tau_b}) \\
&\geq \mathbb E_X (\alpha^b \beta^{n \wedge \tau_b}) \geq \alpha^b \mathbb E_x(\beta^{n \wedge \tau_b}; \tau_b = \infty) \\
&= \alpha^b \beta^n P_X(\tau_b = \infty)
\end{align*}
$$

Letting $n \to \infty$, we infer $P_X(\tau_b = \infty) = 0$.

**Claim.** When $p > \frac{1}{2}$, then $P_x(\tau_a < \infty) = \left(\frac{1}{p}\right)^{x - a}$. 

*Proof.* For $\frac{q}{p} < \alpha < 1$, $0 < \beta< 1$

$$
\begin{align*}
\alpha^X &+ \mathbb E_X(M_{n \wedge \tau_a} ) \\
&= \mathbb E_X(\alpha^{X_n}\beta^n ; n < \tau_a) + \mathbb E_X(\alpha^{X_{\tau_a} \beta^{\tau_a}}; n \geq \tau_a) \\
&\leq \alpha^a \beta^n P_X(n < \tau_a) + \alpha^a\mathbb E_X (\beta^{\tau_a}; \tau_a \leq n ) \\

\end{align*}
$$

The second term can be simplified using the **Monotone Convergence Theorem** -

$$
\begin{align*}
\mathbb E_X (\beta^{\tau_a}; \tau_a < n) &= \mathbb E_X(\beta^{\tau_a}; \tau_a < \infty) \\
&=\alpha^{x - a}
\end{align*}
$$

Letting $\alpha \searrow q/p$, $\beta \nearrow 1$ and

$$
\left(\frac{q}{p}\right)^{x - a} = \mathbb E_x( 1; \tau_a < \infty) = \mathbb P_X(\tau_a < \infty)
$$

In summary, we have for $p > \frac{1}{2}$

$$
\begin{align*}
P_X(\tau_a < \infty) &= \left(\frac{q}{p}\right)^{x - a} < 1\\
P_X(\tau_b < \infty) &= 1
\end{align*}
$$

For $p = \frac{1}{2}$, 

$$
P_X(\tau_b < \infty) = P_X(\tau_a < \infty) = 1
$$

So irrespective of $p$, $P_X(\tau_a \wedge \tau_b < \infty) = 1$. 

#### Example

When $P_X(\tau_a < \tau_b) = \frac{\rho^b - \rho^x}{\rho^b - \rho^a}$ where $M_n = \left(\frac{q}{p}\right)^{X_n} = \rho$ ($p \neq q$)

Note that $M_n = X_n$ when $p = q$. 

Let $\tau = \tau_a \wedge \tau_b$ when $p \neq q$,

$$
\rho^X = \mathbb E_X(M_{n \wedge \tau})
$$

 Using the **Dominated Convergence Theorem**,

$$
\rho^X = \mathbb E_X(M_\tau)
$$

and we get 

$$
\begin{align*}
\rho^X &= \rho^A P_X(\tau_a < \tau_b) + \rho^b P_x(\tau_b < \tau_a) \\
1 &= P_X(\tau_a < \tau_b) + P_X(\tau_b < \tau_a)
\end{align*}
$$

#### Example

Let $M_n = X^2 - n$, with $M_0 = X^2$. Then, for $p = \frac{1}{2}, \sigma^2 = 1, \mu = 1$, $\tau = \tau_a \wedge \tau_b$, we have

$$
\begin{align*}
X^2 &= \mathbb E_X (X^2_{n \wedge \tau}) - \mathbb E(n \wedge \tau) \\
X^2 + \mathbb E(n \wedge \tau) &=  \mathbb E_X (X^2_{n \wedge \tau}) \\ 
\end{align*}
$$

Letting $n \to \infty$ and using Monotone convergence theorem on the left and Dominated convergence theorem on the right, we get

$$
\begin{align*}
X^2 + \mathbb E_X(\tau) &= \mathbb E_X(X_\tau^2) \\
X^2 + \mathbb E_X(\tau) &= a^2\frac{b - x}{b - a} + b^2 \frac{x - a}{b - a}\\
\end{align*}
$$

resulting in $\mathbb E_X(\tau_a \wedge \tau_b) = (X - a)(b - X)$. 
