3. **Progressively Measurable** - Consider a finite segment of time $0 \leq t \leq T$. Then, a stochastic process $X_t(\omega)$ can be viewed as a function $\Omega \times [0, T] \to \mathbb R$. Then, the integral $\int_{0}^t X_s(\omega)ds$ can be viewed as a marginal integral of a joint function. The fact that $\int_0^t X_s(\omega) ds \in \mathcal F_s$ (the integral is measurable) comes from Fubini's theorem in Measure theory. Specifically, the process $X_t(\omega)$ is on the domain $\Omega \times [0, t]$ and is consequently measurable on $\mathcal F_t \otimes \mathcal B[0, t]$. Here $\mathcal B$ refers to **Borel Measurability**. $(X_t)$ is said to be **adapted** to $(\mathcal F_t)$
   
   
   
   **Claim.** If $X_t$ is *adapted* and $t \to X_t(\omega)$ is left-continuous for all $\omega \in \Omega$, then $X$ is progressively measurable.
   
   
   
   In the previous approach to integrate stochastic processes, we considered $\mathcal L_s$ measurable. Now, we generalise this notion using progressive measurability 
   
   $$
   \mathcal L = \{Y: Y \text{ is progressively measurable and } \mathbb E\left(\int_0^T Y_S^2ds\right) < \infty\}
   $$
   
   A key point to note is that $\mathcal L_s$ is dense in $\mathcal L$. That means, given $Y \in \mathcal L$, there exists a sequence of integrands $(Y^{(n)})_{n \geq 1}$ belonging to $\mathcal L_s$ such that 
   
   $$
   \lim_{n \to \infty} \mathbb E\left[\int_0^T (Y_s - Y_s^{(n)})]^2 ds\right] \to 0
   $$
   
   Since each $(Y^{(n)})$ is continuous and a martingale, we will try to show that $M_t^{(n)} = \int_0^t Y_s^{(n)} dW_s$ is a Cauchy sequence converging to the above value - 
   
   $$
   \begin{align*}
\mathbb E\left[ M_t^{(n)} - M_t^{(m)}\right] &= \mathbb E\left[\int_0^t [Y_s^{(n)} - Y_s^{(m)}]\right] \\
&\leq \mathbb E\left[\int_0^T [Y_s^{(n)} - Y_s^{(m)}]\right] \to 0
\end{align*}
   $$
   
   Therefore, $(M_t^{(n)})_{n \geq 1}$ is Cauchy in $\mathcal L^2(\mathcal F_t)$. Consequently, there exists $M_t \in \mathcal L^w(\mathcal F_t)$ such that $M_t^{(n)} \to M_t$. Then, using Doob's inequality
   
   $$
   \begin{align*}
\mathbb E\left(\sup_{0 \leq t \leq T} \vert M_t^{(n)} - M_t^{(m)}\vert^2 \right) \leq 4 \mathbb E[(M_T^{(n)} - M_T^{(m)})^2]
\end{align*}
   $$
   
   we can say that $(M_t)_{0 \leq t \leq T}$ is a path-continuous martingale and $\mathbb E[M_t^2] = \mathbb E[\int_0^t Y_s^2 ds]$ for all $t \in [0, T]$. 
4.  If $Y \in \mathcal L$ is such that $s \to Y_s(w)$ is left-continuous for all $\omega \in \Omega$ then
   
   $$
   \int_0^t Y_S dW_s = \lim_n \sum_{k = 0}^{n - 1} Y_{\frac{k}{n}t}\left(W_{\frac{k + 1}{n} t} - W_{\frac{k}{n} t}\right)
   $$
   
   is also a limiting sum of Riemann sums.
   
   **Example** - Consider $\int_0^t W_s dW_s$ . Since $W \in \mathcal L$, this is integrable. Then, $\mathbb E(W_s^2) = s$ and
   
   $$
   \mathbb E\left[\int_0^T W_s^2 ds \right] = \int_0^T \mathbb E(W_s^2) ds = \int_0^T sds < \infty
   $$



### Quadratic Variation

Similarly, the following is an approximation to quadratic variation

$$
\lim_{n \to \infty} Q_t^{(n)} = \lim_{n \to \infty} \sum_{k = 0}^{n - 1} (W_{\frac{k + q}{n} t} - W_{\frac{k}{n}t})^2 = t
$$

This is because the increments are independent are from the distribution $\mathcal N(0, \frac{t}{n})$. To get the variance, we have

$$
\mathbb E((Q_t^{(n)})^2 ) = 3n \left(\frac{t}{n}\right)^2 + n(n - 1)\left(\frac{t}{n}\right)^2
$$

implying $Var(Q_t^{(n)}) = \frac{2}{n} t^2 \to 0$ as $n \to \infty$.

Going back to our example, writing the integral as Riemann sums -

$$
\begin{align*}
W_t^2 &= \sum_{k = 0}^{n - 1} (W^2_{\frac{k + 1}{n} t} - W^2_{\frac{k }{n} t})  \quad \because W_0^2 = 0\\
&= 2 \sum_{k =0}^{n - 1} W_{\frac{k}{n}t} (W_{\frac{k + 1}{n} t} - W_{\frac{k }{n} t})  + Q_t^{(n)}\quad \because \text{telescopic sum} \\
&= 2\int_0^t W_S dW_s + t
\end{align*}
$$

since the above is left-continuous, letting $n \to \infty$, we get the above expression. The above expression in reminiscent of the fundamental theorem of calculus. Using this, we now state the following theorem

**Theorem (Ito's Formula/Lemma)** For a function $f \in C^2$ and $\vert f'(x) \vert \leq c_0 e^{c_1\vert x \vert}$ for constants $c_0, c_1$, 

$$
f(W_t) = f(W_0) + \int_0^t f'(W_s)sW_s + \frac{1}{2} \int_0^t f"(W_S) ds
$$

This is sort of the fundamental theorem for stochastic calculus. 


