By Ito's formula,

$$
\frac{dS^*_t}{S_t^*} = \sigma\left\{dW_t + \underbrace{\frac{\mu - r}{\sigma}}_{\theta} dt \right\}
$$

Using Girsanov's theorem with $$H_s = - \theta$$, $$P^* = \Lambda_t P$$ is an EMM. 

$$
S_t^* = S_0 + \int_0^t S_u^* d \tilde W_u
$$

so $$S_t^*$$ is a local martingale. Furthermore,

$$
\begin{align*}
\mathbb E^*((S_t^*)^2) &= \mathbb E^*(\exp(2\sigma \tilde W_t - \sigma^2 t))S_0^2. \\
&= e^{4\sigma^2 t/2 - \sigma^2 t}S_0^2 = S_0^2 e^{\sigma^2t}
\end{align*}
$$

Consequently,

$$
\mathbb E^*[\int_0^T (S_t^*)^2 dt]  = S_0^2 \int_0^T e^{\sigma^2 t}dt = S_0^2 \frac{e^{\sigma^2T} - 1} {\sigma^2} < \infty
$$

implying that $$S_t^* \in \mathcal L_{loc}(P^*)$$ and $$(S_t^*)$$ is a $$P^*$$-martingale.

**Corollary** If $$\phi$$ is a self-financing trading strategy, then $$V_t^*(\phi)$$ is a $$p^*$$-local martingale.

*Proof.* 

$$
\begin{align*}
V_t^*(\phi) &= V_0(\phi) + \int_0^t \alpha_u dS_u^* \\
&= V_0(\phi) + \int_0^t (\alpha_u S_u^*) d\tilde W_u
\end{align*}
$$

and $$\alpha_uS_u^* \in \mathcal L_{loc}(P^*)$$ by path continuity.

**Definition.** A self-financing trading strategy is **admissible** provided $$V_t^*(\phi)$$ is a $$P^*$$-martingale (not just a local martingale). 

Also, if $$\mathbb E^*[\int_0^T \alpha_s^2 (S_s^*)^2ds < \infty$$, then $$\phi$$ is admissible.

## Martingale Representation Theorem

If $$(M_t)$$ is a $$P^*$$-martingale (such that $$t \to M_t$$ is right continuous) then there exists a unique $$\eta = (\eta_t)_{0 \leq t \leq T} \in \mathcal L_{loc}$$ such that 

$$
M_t = M_0 + \int_0^t \eta_s d\tilde W_s, 0 \leq t \leq T
$$

**Corollary.** Given $$X \in L^1(\mathcal F_T, P^*)$$, there is a unique admissible $$\phi$$ such that $$\mathbb E^*(X^* \vert \mathcal F_t) = V_t^*(\phi)$$ for $$0 \leq t\leq T$$ ($$X^* = e^{-rT} X$$).

*Proof.* Define a right continuous $$P^*$$-martingale $$M$$ by

$$
M_t := \mathbb E^*(X^* \vert \mathcal F_t)
$$

By the martingale representation theorem, there exists a unique $$\eta$$ such that 

$$
M_t = M_0 + \int_0^t \eta_u d \tilde W_u = M_0 + \int_0^t \alpha_u dS_u^*
$$

where $$\alpha_u := \eta_u/S_u^* \in \mathcal L_{loc}$$. Define $$\beta_t := M_t - \alpha_t S_t^*$$ which is continuous. Then, $$\phi := (\alpha_t, \beta_t)$$ is a self-financing trading strategy and

$$
V_t^*(\phi) = \alpha_t S_t^* + \beta_t = M_t 
$$

is a martingale and hence, admissible. Also, 

$$
V_0(\phi) = M_0 = \mathbb E^*[X^* \vert \mathcal F_0] = \mathbb E^*[X^*]
$$

Therefore, **each** $$X \in L^1(P^*)$$ **is replicable**!

## Pricing a European Contingent Claim

**Theorem.** The unique no arbitrage price of the European claim $$X \in L^1 (P^*)$$ is $$V_t(\phi) = e^{-r(T - t)} \mathbb E^*(X \vert \mathcal F_t)$$.

The European call option is given by $$X = (S_T - K)^*$$

Let us compute $$\mathbb E^*(X^* \vert \mathcal F_t)$$ - Firstly, we have

$$
S_T^* = S_t^* \exp(\sigma(\tilde W_T - \tilde W_t) - \frac{\sigma^2}{2} (T - t))
$$

and $$\tilde W_t - \tilde W_t \sim \mathcal N(0, T - t) \perp\!\!\!\perp_{p^*} \mathcal F_t $$. Renaming $$\tilde W_T - \tilde W_t$$ as $$\sqrt{T - t} Z$$ where $$Z \sim \mathcal N(0, 1)$$ - 

$$
\begin{align*}
\mathbb E^*((S^*_T - K^*)^+ \vert \mathcal F_t) &= E[(S_t^*\exp(\sigma Z\sqrt{T - t}  - \frac{\sigma^2}{2}(T - t)) - K^*)^+] \\
\mathbb E^*[g(S_T^*) \vert \mathcal F_t]&= \mathbb E[g(xe^{\alpha z - \alpha^2/2}) \vert \mathcal F_t]

\end{align*}
$$

where $$x = S_t^*$$ and $$\alpha = \sigma \sqrt{T - t}$$. Let us work with this expression. Letting $$\phi(z) = \frac{1}{\sqrt{2\pi}}e^{-z^2/2}$$  we get $$\mathbb E^*[g(S^*_T) \vert \mathcal F_t] = f(S_t^*, t)$$ where

$$
f(x, t) = \int_{-\infty}^{\infty} g(xe^{\alpha z - \alpha^2/2})\phi(z) dz
$$

Now,

$$
g(xe^{\alpha z - \alpha^2/2}) = \begin{cases}
xe^{\alpha z - \alpha^2/2} - K^* & z > l \\
0 & z \leq l
\end{cases}
$$

where $$l = \frac{L}{\alpha} + \frac{\alpha}{2}$$. and $$L = \log(K^*/x)$$. Then, we get $$f(x, t) = (1) + (2) $$ where

$$
\begin{align*}
(1) &= x\int_l^\infty e^{\alpha z - \alpha^2 /2} \phi(z) dz \\
&= x \int_{\tilde l} ^\infty \frac{1}{\sqrt{2\pi}} e^{-y^2/2}dy = x \Phi(\frac{\alpha}{2} - \frac{L}{\alpha}) \\
(2) &= -K^*\int_l^\infty \phi(z) dz \\
&= -K^* \Phi(-l)
\end{align*}
$$

Finally, we get

$$
C^*(t) = f(x, t) = x \Phi\left(\frac{\log{(x/K^*)}}{\sigma \sqrt{T - t}} + \frac{\sigma \sqrt{T - t}}{2}\right) - K^* \Phi\left(\frac{\log(x/K^*)}{\sigma \sqrt{T - t}} - \frac{\sigma \sqrt{T - t}}{2}\right)
$$
