Using this formulation, we will now look at **Asian Call Options**

# Asian Call Option

The contingent claim is given by

$$
X = \left(\frac{1}{T} \int_0^T S_u du - K\right)^+
$$

and obtain $g(y) = (\frac{Y}{T} - K)^+$. The no-arbitrage price is given by the martingale

$$
\begin{align*}
    V_T &= \mathbb E\left[\left(\frac{1}{T} I_T - K\right)^+ {\Huge \vert} \mathcal F_t\right] \\
&= \mathbb E\left[\left(\frac{1}{T} I_t + \frac{1}{T} \int_t^T S_u du- K\right)^+ {\Huge \vert} \mathcal F_t\right] 
\end{align*}
$$

We'll assume $\mu = r = 0$ for simplicity. For stock price processes we have seen that

$$
S_T = S_0 \exp(\sigma W_t - \frac{\sigma^2 T}{2}) = S_t \exp(\sigma(W_T - W_t) - \frac{\sigma^2}{2}(T - t))
$$

So the idea is to factor out $S_t$ this way in the expectation as well

$$
\begin{align*}
    V_T 
&= S_t \mathbb E\left[\left(\frac{1}{T} \int_t^T \frac{S_u}{S_t}du - \left(\frac{K - \frac{1}{T}I_t}{S_t}\right)\right)^+ {\Huge \vert} \mathcal F_t\right] \\
&= S_t \phi(X_t, t)
\end{align*}
$$

where

$$
\begin{align*}
X_t &= \frac{K - \frac{1}{T}I_t}{S_t} \\
\phi(x, t) &= \mathbb E\left[\left(\frac{1}{T} \int_0^{T - t} \hat S_u du - x\right)^+\right] \\
\hat S_u &= \exp(\sigma(W_{u + t} - W_t) - u\sigma^2/2)
\end{align*}
$$

The expectation of this integral is not trivial. Therefore, we resort to representing the equations as a differential equation. We know $V_t = S_t\phi(X_t, t) $ is a martingale from the way it has been constructed. Let us use Ito's formula to represent it. Furthermore, it can be shown that $X_t = S_t^{-1} (K - \frac{1}{T} I_t) $ is an Ito's process. Why? $I_t$ is an Ito's process and $S_t^{-1} = S_0^{-1} \exp(-\sigma W_t + \sigma^2t/2)$ is also an Ito's process - multiplying Ito's processes gives an Ito process. Using Ito's formula -

$$
\begin{align*}
d(S_t^{-1}) &= \frac{1}{S_t} \left(\sigma dW_t + \sigma^2 t\right)\\
dX_t&= -S_t^{-1} \frac{1}{T} S_t dt + (k - \frac{1}{T} I_t ) d(S_t^{-1})
\end{align*}
$$

The quadratic variation of $X_t$ is $0$, and therefore the product rule does not have any covariation terms.

Finally, we get

$$
\begin{align*}
dV_t =  S_t \left[\phi_t - \frac{1}{T} \phi_x + \frac{\sigma^2}{2} X_t^2 \phi_{xx}\right]dt + \text{martingale terms}
\end{align*}
$$

We have

$$
\begin{align*}
\phi(x, T) = (-x)^+ = x^{-} \\
\phi_t - \frac{1}{T} \phi_x + \frac{\sigma^2 x^2}{2}\phi_{xx} = 0
\end{align*}
$$

The stochastic differential equation comes from the fact that $V_t$ is a martingale, and with this we have essentially captured the process in terms of a single spatial random variable. Previously, we had

$$
\mathbb E(g(I_T) \vert \mathcal F_t) = \psi(S_t, I_t, t)
$$

where 

$$
\psi_t + x \psi_y + \frac{\sigma^2 x^2}{2} \psi_{xx} = 0 \\
\psi(x, y, T) = \left(\frac{y}{T} - K\right)^+
$$

In fact, with brutal exercise, we can show that

$$
\psi(x, y, y) = x \phi\left(\frac{TK - y}{xT}, t\right)
$$

Note that we were able to do such a simplification for a specific nature of $g$ - here $g$ is a straight-line function ($g_k(cy) = cg_{k/c}(y)$). Something similar can be done when $g(y) = y^p$ as well.

## Geometric Asian Call

A continual version of geometric mean is given by

$$
G_T = \exp\left(\frac{1}{T}\int_0^T \log S_t dt \right)
$$

So, the contingent claim is given by

$$
\begin{align*}
X &= \left(\exp\left(\frac{1}{T} \int_0^T \log S_u du\right) -K \right)^+ \\
\text{Also}& \log S_u = \log S_0 + \sigma W_u - \frac{\sigma^2u}{u} 
\end{align*}
$$

 Once again, assume $\mu = r = 0$. The no-arbitrage price is given by

$$
\mathbb E[X \vert \mathcal F_t] = \mathbb E\left[\left[S_0\exp\left(\frac{\sigma}{T} J_t + \frac{\sigma}{T}\int_t^TW_u du - \frac{\sigma^2 T}{4}\right) - K\right]^+ {\Huge \vert} \mathcal F_t\right]
$$

where $J_t = \int_0^t W_u du$. Then,

$$
\begin{align*}
\mathbb E[X \vert \mathcal F_t] = \mathbb E\left[\left[S_0\exp\left(\frac{\sigma}{T} J_t + \frac{\sigma}{T}(T-t) W_t + \frac{\sigma}{T}\int_0^{T - t}\hat W_s ds - \frac{\sigma^2 T}{4}\right) - K\right]^+ {\Huge \vert} \mathcal F_t\right]
\end{align*}
$$

where $\hat W_s = W_{t + s} - W_t$ and $\hat J_{T - t} = \int_0^{T - t} \hat W_u du \sim \mathcal N(0, (T - t)^3/3)$

The above expression is then equal to $\psi(W_t, J_t, t)$

where

$$
\psi(x, y, y) = \mathbb E\left[\left(S_0 \exp\left(\frac{\sigma}{T} y + \frac{\sigma}{T}(T - t) x - \frac{\sigma^2T}{4} + \frac{\sigma}{T} \hat J_{T - t}\right) - K \right)^+\right]
$$

this is very similar to the expectation we have in Black-Scholes - $\mathbb E[(x \exp(\alpha x - \frac{\alpha^2}{2}) - K)^+]$. 
